FiatFormal/Language/Exp.v
@@ -59,20 +59,20 @@ Inductive wfX : tyenv -> exp -> Prop :=
    -> Forall (wfA te) alts
    -> wfX te (XMatch x alts)
 
- (* | WfX_XChoice *)
- (*   : forall te t1 fp, *)
- (*   , wfX te (XChoice t1 fp)
-(* TODO: consider uses of this, if they exist *) *)
- (* | WfX_XChoice : forall te t11 fp xs, get 0 (Predtypes fp) = Some t11 *)
- (*                                 -> length (skipn 1 (Predtypes fp)) = length xs *)
- (*                                 -> wfX te (XChoice t11 xs fp) *)
- (* | WfX_XCall *)
- (*   : forall ds x ts te xs ac n, *)
- (*     getADTMethodBody ac n ds  = Some x *)
- (*     -> getADTMethodSig ac n ds = Some ts *)
- (*     -> wfX (delete ((length ts) - 1) ts) x (* Having appropriate size of tyenv all the matters here *) *)
- (*     -> Forall (wfX te) xs *)
- (*     -> wfX te (XCall ac n xs) *)
+ | WfX_XChoice
+   : forall te t1 xs fp,
+     Forall (wfX te) xs
+     -> wfX te (XChoice t1 xs fp)
+
+ | WfX_XCall
+   : forall adt_ds x s te ac n xs,
+     getADTBody ac n adt_ds  = Some x
+     -> getADTSig ac n adt_ds = Some s
+     (* Having appropriate size of tyenv all the matters here *)
+     -> wfX (buildMethodTyEnv (TAdt ac) s) x
+     -> length xs = s.(arity) + length(s.(dom))
+     -> Forall (wfX te) xs
+     -> wfX te (XCall ac n xs)
 
 with    wfA : tyenv -> alt -> Prop :=
  | WfA_AAlt
