FiatFormal/Language/Progress.v
@@ -4,89 +4,91 @@ Require Import FiatFormal.Language.TyJudge.
 Require Import FiatFormal.Language.Exp.
 
 Theorem fiatProgress
-  : forall ds x t,
-    TYPE ds nil x t
-    -> value x \/ (exists x', STEP x x') \/ Xhas_choice x.
+  : forall alg_ds adt_ds x t,
+    TYPE alg_ds adt_ds nil x t
+    -> value x \/ (exists x', STEP adt_ds x x') \/ Xhas_choice adt_ds x.
 Proof.
-  Admitted.
+ intros. gen t.
+ induction x using exp_mutind with
+     (PA := fun a => a = a)
+     (PF := fun f => f = f); rip; burn.
 
-(* A well typed expression is either a well formed value,
-   or can transition to the next state. *)
-Theorem progress
- :  forall ds x t
- ,  TYPE ds nil x t
- -> value x \/ (exists x', STEP x x').
-Proof.
-(*  intros. gen t. *)
-(*  induction x using exp_mutind with *)
-(*   (PA := fun a => a = a); rip; burn. *)
+ Case "XApp".
+  right; left.
+  inverts_type.
+  edestruct IHx1; eauto.
+  SCase "value x1".
+   edestruct IHx2; eauto.
+   SSCase "value x2".
 
-(*  Case "XApp". *)
-(*   right. *)
-(*   inverts_type. *)
-(*   edestruct IHx1; eauto. *)
-(*   SCase "value x1". *)
-(*    edestruct IHx2; eauto. *)
-(*    SSCase "value x2". *)
-(*     have HF: (exists t x, x1 = XLam t x). *)
-(*      destruct HF as [t11]. *)
-(*      destruct H1 as [x12]. *)
-(*      subst. *)
-(*      exists (substX 0 x2 x12). *)
-(*      eauto. *)
-(*     SSCase "x2 steps". *)
-(*      destruct H0 as [x2']. *)
-(*      exists (XApp x1 x2'). auto. *)
-(*   SCase "x1 steps". *)
-(*    destruct H  as [x1']. *)
-(*    exists (XApp x1' x2). *)
-(*    eapply (EsContext (fun xx => XApp xx x2)); auto. *)
+   (* next statement fails because XLam is not unique in the type (TFun _ _) *)
+    have HF: (exists t x, x1 = XLam t x).
+     destruct HF as [t11].
+     destruct H1 as [x12].
+     subst.
+     exists (substX 0 x2 x12).
+     eauto.
+    SSCase "x2 steps".
+     destruct H0 as [x2'].
+     exists (XApp x1 x2'). auto.
+  SCase "x1 steps".
+   destruct H  as [x1'].
+   exists (XApp x1' x2).
+   eapply (EsContext (fun xx => XApp xx x2)); auto.
 
-(*  Case "XCon". *)
-(*   inverts_type. *)
+ Case "XCon".
+  inverts_type.
 
-(*   (* All ctor args are either wnf or can step *) *)
-(*   assert (Forall (fun x => wnfX x \/ (exists x', STEP x x')) xs) as HWS. *)
-(*    norm. rip. *)
-(*    have (exists t, TYPE ds nil x t). dest t. *)
-(*    have (value x \/ (exists x', STEP x x')). *)
-(*    inverts H2; burn. *)
+  (* All ctor args are either wnf or can step *)
+  assert (Forall (fun x => wnfX x \/ (exists x', STEP x x')) xs) as HWS.
+   norm. rip.
+   have (exists t, TYPE ds nil x t). dest t.
+   have (value x \/ (exists x', STEP x x')).
+   inverts H2; burn.
 
-(*   (* All ctor args are wnf, or there is a context where one can step *) *)
-(*   lets D: (@exps_ctx_run exp exp) HWS. *)
-(*   inverts D. *)
-(*    (* All ctor args are wnf *) *)
-(*    left. eauto 6. *)
-(*    (* There is a context where one ctor arg can step *) *)
-(*    right. *)
-(*     dest C. dest x'. *)
-(*     rip. *)
-(*     lets D: step_context_XCon_exists H1 H5. *)
-(*     destruct D as [x'']. eauto. *)
+  (* All ctor args are wnf, or there is a context where one can step *)
+  lets D: (@exps_ctx_run exp exp) HWS.
+  inverts D.
+   (* All ctor args are wnf *)
+   left. eauto 6.
+   (* There is a context where one ctor arg can step *)
+   right.
+    dest C. dest x'.
+    rip.
+    lets D: step_context_XCon_exists H1 H5.
+    destruct D as [x'']. eauto.
 
-(*  Case "XCase". *)
-(*   right. *)
-(*   inverts_type. *)
-(*   have HS: (value x \/ (exists x', STEP x x')). *)
-(*   inverts HS. clear IHx. *)
-(*   SCase "x value". *)
-(*    destruct x; nope. *)
-(*     SSCase "XCon". *)
-(*      inverts_type. *)
-(*      rrwrite (dcs0 = dcs). *)
-(*      have HG: (exists ts x, getAlt d aa = Some (AAlt d ts x)) *)
-(*       by burn using getAlt_exists. *)
-(*      dest ts. dest x. *)
-(*      exists (substXs 0 l x). *)
-(*      burn. *)
+ Case "XCase".
+  right.
+  inverts_type.
+  have HS: (value x \/ (exists x', STEP x x')).
+  inverts HS. clear IHx.
+  SCase "x value".
+   destruct x; nope.
+    SSCase "XCon".
+     inverts_type.
+     rrwrite (dcs0 = dcs).
+     have HG: (exists ts x, getAlt d aa = Some (AAlt d ts x))
+      by burn using getAlt_exists.
+     dest ts. dest x.
+     exists (substXs 0 l x).
+     burn.
 
-(*   SCase "x steps". *)
-(*    destruct H0 as [x']. *)
-(*    exists (XCase x' aa). *)
-(*    lets D: EsContext XcCase; eauto. *)
-(* Qed. *)
+  SCase "x steps".
+   destruct H0 as [x'].
+   exists (XCase x' aa).
+   lets D: EsContext XcCase; eauto.
+Qed.
+Admitted.
 
 (* ORIG *)
+(* A well typed expression is either a well formed value,
+   or can transition to the next state. *)
+(* Theorem progress *)
+(*  :  forall ds x t *)
+(*  ,  TYPE ds nil x t *)
+(*  -> value x \/ (exists x', STEP x x'). *)
+(* Proof. *)
 (*  intros. gen t. *)
 (*  induction x using exp_mutind with  *)
 (*   (PA := fun a => a = a); rip; burn. *)
@@ -155,4 +157,4 @@ Proof.
 (*    exists (XCase x' aa). *)
 (*    lets D: EsContext XcCase; eauto. *)
 (* Qed. *)
-Admitted.
+(* Admitted. *)
