FiatFormal/Language/StepAlt.v
@@ -7,10 +7,10 @@ Require Export FiatFormal.Language.SubstExpExp.
 (* The body of an alternative is well typed under an environment
    that includes the arguments of the constructor being matched. *)
 Lemma getAlt_bodyIsWellTyped_fromAlts
- :  forall ds te tPat tResult alts dc tsArgs x
- ,  Forall (fun a => TYPEA ds te a tPat tResult) alts
+  : forall alg_ds adt_ds te tPat tResult alts dc tsArgs x,
+    Forall (fun a => TYPEA alg_ds adt_ds te a tPat tResult) alts
  -> In (AAlt dc tsArgs x) alts
- -> TYPE ds (te >< tsArgs) x tResult.
+ -> TYPE alg_ds adt_ds (te >< tsArgs) x tResult.
 Proof.
 (*  intros.  *)
 (*  norm. spec H H0.  *)
@@ -22,11 +22,11 @@ Admitted.
    under an environment that includes the arguments of the constructor
    being matched. *)
 Lemma getAlt_bodyIsWellTyped_fromCase
- :  forall ds te tResult tCon alts dc tsArgs x1 x2
- ,  TYPE ds te (XMatch x1 alts) tResult
- -> getDataDef dc ds   = Some (DefData dc tsArgs tCon)
- -> getAlt     dc alts = Some (AAlt    dc tsArgs x2)
- -> TYPE ds (te >< tsArgs) x2 tResult.
+  : forall alg_ds adt_ds te tResult tCon alts dc tsArgs x1 x2,
+    TYPE alg_ds adt_ds te (XMatch x1 alts) tResult
+    -> getDataDef dc alg_ds = Some (DefData dc tsArgs tCon)
+    -> getAlt     dc alts   = Some (AAlt    dc tsArgs x2)
+    -> TYPE alg_ds adt_ds (te >< tsArgs) x2 tResult.
 Proof.
 (*  intros. *)
 (*  inverts keep H. *)
@@ -40,11 +40,11 @@ Admitted.
 (* If an alternative is well typed then the types of the ctor
    args embedded in it match those in the data type definition *)
 Lemma getAlt_ctorArgTypesMatchDataDef
- :  forall ds te tCon tResult alts dc x tsArgs tsArgs'
- ,  Forall (fun alt => TYPEA ds te alt tCon tResult) alts
- -> getDataDef dc ds = Some (DefData dc tsArgs  tCon)
- -> getAlt dc alts   = Some (AAlt    dc tsArgs' x)
- -> tsArgs = tsArgs'.
+  : forall alg_ds adt_ds te tCon tResult alts dc x tsArgs tsArgs',
+    Forall (fun alt => TYPEA alg_ds adt_ds te alt tCon tResult) alts
+    -> getDataDef dc alg_ds = Some (DefData dc tsArgs  tCon)
+    -> getAlt dc alts       = Some (AAlt    dc tsArgs' x)
+    -> tsArgs = tsArgs'.
 Proof.
 (*  intros. norm. *)
 (*  lets D: getAlt_in H1. spec H D. *)
